verified/Smtlink.lisp
@@ -14,1057 +14,1252 @@
 (include-book "SMT-verified-cps")
 (include-book "SMT-config")
 
-;; (defsection Smtlink-process-user-hint
-;;   :parents (Smtlink)
-;;   :short "Functionalities for processing user hints given to Smtlink. User
-;;   hints will be merged with (smt-hint)."
+(defsection Smtlink-process-user-hint
+  :parents (Smtlink)
+  :short "Functionalities for processing user hints given to Smtlink. User
+  hints will be merged with (smt-hint)."
 
   ;; --------------------------------------------------------
 
-;; Example:
-;; :hints (("Goal"
-;;          :clause-processor
-;;          (SMT::smtlink clause
-;;                        '(:functions ((f0 :formals ((a0 rationalp))
-;;                                          :returns (r0 rationalp :hints (:use ((:instance returns-lemma))))
-;;                                          :level 1
-;;                                          :guard ((> a0 0) :hints (:use ((:instance guard-lemma))))
-;;                                          :more-returns ((> r0 0) :hints (:use ((:instance more-lemma))))))
-;;                          :hypothesis (((> a b) :hints (:use ((:instance lemma)))))
-;;                          :main-hint (:use ((:instance thm1)))
-;;                          :int-to-rat nil
-;;                          :smt-fname ""
-;;                          :rm-file t
-;;                          :smt-solver-params (...)
-;;                          :smt-solver-cnf ()))))
+  ;; Example:
+  ;; :hints (("Goal"
+  ;;          :clause-processor
+  ;;          (SMT::smtlink clause
+  ;;                        '(:functions ((f0 :formals ((a0 rationalp))
+  ;;                                          :returns (r0 rationalp :hints (:use ((:instance returns-lemma))))
+  ;;                                          :level 1
+  ;;                                          :guard ((> a0 0) :hints (:use ((:instance guard-lemma))))
+  ;;                                          :more-returns (((> r0 0) :hints (:use ((:instance more-lemma)))))))
+  ;;                          :hypothesis (((> a b) :hints (:use ((:instance lemma)))))
+  ;;                          :main-hint (:use ((:instance thm1)))
+  ;;                          :int-to-rat nil
+  ;;                          :smt-fname ""
+  ;;                          :rm-file t
+  ;;                          :smt-solver-params (...)
+  ;;                          :smt-solver-cnf ()))))
 
-;; Types:
-;; qbooleanp/fix
-;; qnatp/fix
-;; qstringp/fix
-;; hints-syntax-p/fix
-;; hypothesis-syntax-p/fix
-;; hypothesis-lst-syntax-p/fix
-;; argument-syntax-p/fix
-;; argument-lst-syntax-p/fix
-;; function-option-syntax-p/fix
-;; function-option-lst-syntax-p/fix
-;; function-syntax-p/fix
-;; function-lst-syntax-p/fix
-;; smt-solver-cnf-p/fix
-;; smt-solver-params-p/fix
-;; smtlink-hint-syntax-p/fix
+  ;; Types:
+  ;; qbooleanp/fix
+  ;; qnatp/fix
+  ;; qstringp/fix
+  ;; hints-syntax-p/fix
+  ;; hypothesis-syntax-p/fix
+  ;; hypothesis-lst-syntax-p/fix
+  ;; argument-syntax-p/fix
+  ;; argument-lst-syntax-p/fix
+  ;; function-option-syntax-p/fix
+  ;; function-option-lst-syntax-p/fix
+  ;; function-syntax-p/fix
+  ;; function-lst-syntax-p/fix
+  ;; smt-solver-cnf-p/fix
+  ;; smt-solver-params-p/fix
+  ;; smtlink-hint-syntax-p/fix
 
-(define qstringp ((term t))
-  :returns (syntax-good? booleanp)
-  :short "Recognizer for a quoted stringp."
-  (and (true-listp term)
-       (equal (len term) 2)
-       (equal (car term) 'quote)
-       (stringp (cadr term))))
+  (define qstringp ((term t))
+    :returns (syntax-good? booleanp)
+    :short "Recognizer for a quoted stringp."
+    (and (true-listp term)
+         (car term) (cadr term) (not (cddr term))
+         (equal (car term) 'quote)
+         (stringp (cadr term))))
 
-(define qstring-fix ((term qstringp))
-  :short "Fixing function for a qstringp."
-  :returns (fixed-term qstringp)
-  (mbe :logic (if (qstringp term) term ''"")
-       :exec term))
+  (define qstring-fix ((term qstringp))
+    :short "Fixing function for a qstringp."
+    :returns (fixed-term qstringp)
+    (mbe :logic (if (qstringp term) term ''"")
+         :exec term))
 
-(defthm qstring-fix-idempotent-lemma
-  (equal (qstring-fix (qstring-fix x))
-         (qstring-fix x))
-  :hints (("Goal" :in-theory (enable qstring-fix))))
+  (defthm qstring-fix-idempotent-lemma
+    (equal (qstring-fix (qstring-fix x))
+           (qstring-fix x))
+    :hints (("Goal" :in-theory (enable qstring-fix))))
 
-;; This one shows that it's possible to connect fixing function and
-;; the type functions together, and became useful for other defprods, etc.
-;; Since I'm currently not using defprods for others either, this is probably
-;; not that useful. However, this deffixtype shows as an example for future
-;; necessity.
-(deffixtype qstring
-  :pred  qstringp
-  :fix   qstring-fix
-  :equiv qstring-equiv
-  :define t
-  :forward t
-  :topic qstringp)
+  ;; This one shows that it's possible to connect fixing function and
+  ;; the type functions together, and became useful for other defprods, etc.
+  ;; Since I'm currently not using defprods for others either, this is probably
+  ;; not that useful. However, this deffixtype shows as an example for future
+  ;; necessity.
+  (deffixtype qstring
+    :pred  qstringp
+    :fix   qstring-fix
+    :equiv qstring-equiv
+    :define t
+    :forward t
+    :topic qstringp)
 
-(define qnatp ((term t))
-  :returns (syntax-good? booleanp)
-  :short "Recognizer for a quoted qnatp."
-  (and (true-listp term)
-       (equal (len term) 2)
-       (equal (car term) 'quote)
-       (natp (cadr term))))
+  (define qnatp ((term t))
+    :returns (syntax-good? booleanp)
+    :short "Recognizer for a quoted qnatp."
+    (and (true-listp term)
+         (car term) (cadr term) (not (cddr term))
+         (equal (car term) 'quote)
+         (natp (cadr term))))
 
-(define qnat-fix ((term qnatp))
-  :returns (fixed-term qnatp)
-  :short "Fixing function for a qnatp."
-  (mbe :logic (if (qnatp term) term ''0)
-       :exec term))
+  (define qnat-fix ((term qnatp))
+    :returns (fixed-term qnatp)
+    :short "Fixing function for a qnatp."
+    (mbe :logic (if (qnatp term) term ''0)
+         :exec term))
 
-(define qbooleanp ((term t))
-  :short "Recognizer for a quoted booleanp."
-  :returns (syntax-good? booleanp)
-  (and (true-listp term)
-       (equal (len term) 2)
-       (equal (car term) 'quote)
-       (booleanp (cadr term))))
+  (defthm qnat-fix-idempotent-lemma
+    (equal (qnat-fix (qnat-fix x))
+           (qnat-fix x))
+    :hints (("Goal" :in-theory (enable qnat-fix))))
 
-(define qboolean-fix ((term qbooleanp))
-  :returns (fixed-term qbooleanp)
-  :short "Fixing function for a qbooleanp."
-  (mbe :logic (if (qbooleanp term) term ''nil)
-       :exec term))
+  (deffixtype qnat
+    :pred  qnatp
+    :fix   qnat-fix
+    :equiv qnat-equiv
+    :define t
+    :forward t
+    :topic qnatp)
 
-(define hints-syntax-p ((term t))
-  :returns (syntax-good? booleanp)
-  :short "Recognizer for hints-syntax."
-  (true-listp term))
+  (define qbooleanp ((term t))
+    :short "Recognizer for a quoted booleanp."
+    :returns (syntax-good? booleanp)
+    (and (true-listp term)
+         (car term)
+         (equal (car term) 'quote)
+         (booleanp (cadr term))))
 
-(define hints-syntax-fix ((term hints-syntax-p))
-  :returns (fixed-term hints-syntax-p)
-  :short "Fixing function for a hints-sytnax-p."
-  (mbe :logic (if (hints-syntax-p term) term nil)
-       :exec term))
+  (define qboolean-fix ((term qbooleanp))
+    :returns (fixed-term qbooleanp)
+    :short "Fixing function for a qbooleanp."
+    (mbe :logic (if (qbooleanp term) term ''nil)
+         :exec term))
 
-(define hypothesis-syntax-p ((term t))
-  :returns (syntax-good? booleanp)
-  :short "Recognizer for hypothesis-syntax."
-  (or (and (atom term)
-           (equal term nil))
-      ;; Without hints
-      (and (true-listp term)
-           (equal (len term) 1)
-           (pseudo-termp (car term)))
-      ;; With hints
-      (and (true-listp term)
-           (equal (len term) 3)
-           (pseudo-termp (car term))
-           (equal (cadr term) ':hints)
-           (hints-syntax-p (caddr term))))
-  ///
-  (defthm true-listp-of-caddr
-    (implies
-     (and (consp term)
-          (consp (cdr term))
-          (true-listp (cddr term))
-          (equal (+ 2 (len (cddr term))) 3)
-          (pseudo-termp (car term))
-          (equal (cadr term) :hints)
-          (hints-syntax-p (caddr term)))
-     (true-listp (caddr term)))
-    :hints (("Goal" :in-theory (enable hints-syntax-p)))))
+  (defthm qboolean-fix-idempotent-lemma
+    (equal (qboolean-fix (qboolean-fix x))
+           (qboolean-fix x))
+    :hints (("Goal" :in-theory (enable qboolean-fix))))
 
-(define hypothesis-syntax-fix ((term hypothesis-syntax-p))
-  :returns (fixed-term hypothesis-syntax-p)
-  :short "Fixing function for a hypothesis-syntax-p."
-  (mbe :logic (if (hypothesis-syntax-p term) term nil)
-       :exec term))
+  (deffixtype qboolean
+    :pred  qbooleanp
+    :fix   qboolean-fix
+    :equiv qboolean-equiv
+    :define t
+    :forward t
+    :topic qbooleanp)
 
-(define hypothesis-lst-syntax-p ((term t))
-  :returns (syntax-good? booleanp)
-  :short "Recognizer for hypothesis-lst-syntax."
-  (b* (((if (atom term)) (equal term nil))
-       ((cons first rest) term))
-    (and (hypothesis-syntax-p first)
-         (hypothesis-lst-syntax-p rest))))
+  (define hints-syntax-p ((term t))
+    :returns (syntax-good? booleanp)
+    :short "Recognizer for hints-syntax."
+    (true-listp term))
 
-(define hypothesis-lst-syntax-fix ((term hypothesis-lst-syntax-p))
-  :returns (fixed-term hypothesis-lst-syntax-p
-                       :hints (("Goal"
-                                :in-theory (enable hypothesis-lst-syntax-p))))
-  :verify-guards nil
-  :short "Fixing function for a hypothesis-lst-syntax-p."
-  (mbe :logic (if (consp term)
-                  (cons (hypothesis-syntax-fix (car term))
-                        (hypothesis-lst-syntax-fix (cdr term)))
-                nil)
-       :exec term))
+  (define hints-syntax-fix ((term hints-syntax-p))
+    :returns (fixed-term hints-syntax-p)
+    :short "Fixing function for a hints-sytnax-p."
+    (mbe :logic (if (hints-syntax-p term) term nil)
+         :exec term))
 
-(verify-guards hypothesis-lst-syntax-fix
-  :hints (("Goal" :in-theory (enable hypothesis-syntax-fix
-                                     hypothesis-lst-syntax-p hypothesis-lst-syntax-fix))))
+  (define hypothesis-syntax-p ((term t))
+    :returns (syntax-good? booleanp)
+    :short "Recognizer for hypothesis-syntax."
+    (or (and (atom term)
+             (equal term nil))
+        ;; Without hints
+        (and (true-listp term)
+             (car term) (not (cdr term))
+             (pseudo-termp (car term)))
+        ;; With hints
+        (and (true-listp term)
+             (car term) (cadr term) (not (cdddr term))
+             (pseudo-termp (car term))
+             (equal (cadr term) ':hints)
+             (hints-syntax-p (caddr term))))
+    ///
+    (defthm true-listp-of-caddr
+      (implies
+       (and (consp term)
+            (consp (cdr term))
+            (true-listp (cddr term))
+            (equal (+ 2 (len (cddr term))) 3)
+            (pseudo-termp (car term))
+            (equal (cadr term) :hints)
+            (hints-syntax-p (caddr term)))
+       (true-listp (caddr term)))
+      :hints (("Goal" :in-theory (enable hints-syntax-p)))))
 
-(defthm hypothesis-lst-syntax-fix-idempotent-lemma
-  (equal (hypothesis-lst-syntax-fix (hypothesis-lst-syntax-fix x))
-         (hypothesis-lst-syntax-fix x))
-  :hints (("Goal" :in-theory (enable hypothesis-lst-syntax-fix hypothesis-syntax-fix))))
+  (define hypothesis-syntax-fix ((term hypothesis-syntax-p))
+    :returns (fixed-term hypothesis-syntax-p)
+    :short "Fixing function for a hypothesis-syntax-p."
+    (mbe :logic (if (hypothesis-syntax-p term) term nil)
+         :exec term))
 
-(deffixtype hypothesis-lst-syntax
-  :pred  hypothesis-lst-syntax-p
-  :fix   hypothesis-lst-syntax-fix
-  :equiv hypothesis-lst-syntax-equiv
-  :define t
-  :forward t
-  :topic hypothesis-lst-syntax-p)
+  (defthm hypothesis-syntax-fix-idempotent-lemma
+    (equal (hypothesis-syntax-fix (hypothesis-syntax-fix x))
+           (hypothesis-syntax-fix x))
+    :hints (("Goal" :in-theory (enable hypothesis-syntax-fix))))
 
-(define smt-typep ((term t))
-  :returns (valid-type? booleanp)
-  :short "Types allowed in Smtlink."
-  (if (member-equal term
-                    ' (rationalp realp rational/realp booleanp integerp))
-      t nil))
+  (deffixtype hypothesis-syntax
+    :pred  hypothesis-syntax-p
+    :fix   hypothesis-syntax-fix
+    :equiv hypothesis-syntax-equiv
+    :define t
+    :forward t
+    :topic hypothesis-syntax-p)
 
-(define argument-syntax-p ((term t))
-  :returns (syntax-good? booleanp)
-  :short "Recognizer for argument-syntax."
-  (or (and (atom term)
-           (equal term nil))
-      ;; Just the name
-      (and (true-listp term)
-           (equal (len term) 1)
-           (symbolp (car term)))
-      ;; The name and the type/guard
-      (and (true-listp term)
-           (equal (len term) 2)
-           (smt-typep (car term))
-           (pseudo-termp (cadr term)))
-      ;; The name, the type and the :hints
-      (and (true-listp term)
-           (equal (len term) 3)
-           (symbolp (car term))
-           (smt-typep (cadr term))
-           (hints-syntax-p (cddr term)))))
+  (define hypothesis-lst-syntax-p ((term t))
+    :returns (syntax-good? booleanp)
+    :short "Recognizer for hypothesis-lst-syntax."
+    (b* (((if (atom term)) (equal term nil))
+         ((cons first rest) term))
+      (and (hypothesis-syntax-p first)
+           (hypothesis-lst-syntax-p rest)))
+    ///
+    (defthm true-listp-of-hypothesis-lst-syntax
+      (implies (hypothesis-lst-syntax-p x)
+               (true-listp x))))
 
-(define argument-syntax-fix ((term argument-syntax-p))
-  :returns (fixed-term argument-syntax-p)
-  :short "Fixing function for argument-syntax-p."
-  (mbe :logic (if (argument-syntax-p term) term nil)
-       :exec term))
+  (define hypothesis-lst-syntax-fix ((term hypothesis-lst-syntax-p))
+    :returns (fixed-term hypothesis-lst-syntax-p
+                         :hints (("Goal"
+                                  :in-theory (enable hypothesis-lst-syntax-p))))
+    :verify-guards nil
+    :short "Fixing function for a hypothesis-lst-syntax-p."
+    (mbe :logic (if (consp term)
+                    (cons (hypothesis-syntax-fix (car term))
+                          (hypothesis-lst-syntax-fix (cdr term)))
+                  nil)
+         :exec term))
 
-(define argument-lst-syntax-p ((term t))
-  :short "Recognizer for argument-lst-syntax."
-  :returns (syntax-good? booleanp)
-  (b* (((if (atom term)) (equal term nil))
-       ((cons first rest) term))
-    (and (argument-syntax-p first)
-         (argument-lst-syntax-p rest))))
+  (verify-guards hypothesis-lst-syntax-fix
+    :hints (("Goal" :in-theory (enable hypothesis-syntax-fix
+                                       hypothesis-lst-syntax-p hypothesis-lst-syntax-fix))))
 
-(define argument-lst-syntax-fix ((term argument-lst-syntax-p))
-  :short "Fixing function for argument-lst-syntax."
-  :returns (fixed-term argument-lst-syntax-p
-                       :hints (("Goal"
-                                :in-theory (enable argument-lst-syntax-p))))
-  :verify-guards nil
-  (mbe :logic (if (consp term)
-                  (cons (argument-syntax-fix (car term))
-                        (argument-lst-syntax-fix (cdr term)))
-                nil)
-       :exec term))
-(verify-guards argument-lst-syntax-fix
-  :hints (("Goal"
-           :in-theory (enable argument-lst-syntax-fix argument-syntax-fix argument-lst-syntax-p))))
+  (defthm hypothesis-lst-syntax-fix-idempotent-lemma
+    (equal (hypothesis-lst-syntax-fix (hypothesis-lst-syntax-fix x))
+           (hypothesis-lst-syntax-fix x))
+    :hints (("Goal" :in-theory (enable hypothesis-lst-syntax-fix hypothesis-syntax-fix))))
 
-(defconst *function-options*
-  '((:formals . argument-lst-syntax-p)
-    (:returns . argument-lst-syntax-p)
-    (:level . qnatp)
-    (:guard . hypothesis-lst-syntax-p)
-    (:more-returns . hypothesis-lst-syntax-p)))
+  (deffixtype hypothesis-lst-syntax
+    :pred  hypothesis-lst-syntax-p
+    :fix   hypothesis-lst-syntax-fix
+    :equiv hypothesis-lst-syntax-equiv
+    :define t
+    :forward t
+    :topic hypothesis-lst-syntax-p)
 
-(defconst *function-option-names*
-  (strip-cars *function-options*))
+  (define smt-typep ((term t))
+    :returns (valid-type? booleanp)
+    :short "Types allowed in Smtlink."
+    (if (member-equal term
+                      ' (rationalp realp rational/realp booleanp integerp))
+        t nil))
 
-(defconst *function-option-types*
-  (remove-duplicates-equal (strip-cdrs *function-options*)))
+  (define argument-syntax-p ((term t))
+    :returns (syntax-good? booleanp)
+    :short "Recognizer for argument-syntax."
+    (or (and (atom term)
+             (equal term nil))
+        ;; Just the name
+        (and (true-listp term)
+             (car term) (not (cdr term))
+             (symbolp (car term)))
+        ;; The name and the type/guard
+        (and (true-listp term)
+             (car term) (cadr term) (not (cddr term))
+             (smt-typep (car term))
+             (symbolp (cadr term)))
+        ;; The name, the type and the :hints
+        (and (true-listp term)
+             (car term) (cadr term) (not (cdddr term)) 
+             (symbolp (car term))
+             (smt-typep (cadr term))
+             (hints-syntax-p (cddr term)))))
 
-(define function-option-type-p ((option-type t))
-  :returns (syntax-good? booleanp)
-  :short "Recoginizer for function-option-type."
-  (if (member-equal option-type *function-option-types*) t nil))
+  (define argument-syntax-fix ((term argument-syntax-p))
+    :returns (fixed-term argument-syntax-p)
+    :short "Fixing function for argument-syntax-p."
+    (mbe :logic (if (argument-syntax-p term) term nil)
+         :exec term))
 
-(define function-option-type-fix ((option-type function-option-type-p))
-  :returns (fixed-option-type function-option-type-p
-                              :hints (("Goal" :in-theory (enable
-                                                          function-option-type-p ))))
-  :short "Fixing function for function-option-type."
-  (mbe :logic (if (function-option-type-p option-type) option-type 'qnatp)
-       :exec option-type))
+  (define argument-lst-syntax-p ((term t))
+    :short "Recognizer for argument-lst-syntax."
+    :returns (syntax-good? booleanp)
+    (b* (((if (atom term)) (equal term nil))
+         ((cons first rest) term))
+      (and (argument-syntax-p first)
+           (argument-lst-syntax-p rest))))
 
-(define function-option-name-p ((option-name t))
-  :returns (syntax-good? booleanp)
-  :short "Recoginizer for an function-option-name."
-  (if (member-equal option-name *function-option-names*) t nil))
+  (defthm argument-syntax-fix-idempotent-lemma
+    (equal (argument-syntax-fix (argument-syntax-fix x))
+           (argument-syntax-fix x))
+    :hints (("Goal" :in-theory (enable argument-syntax-fix))))
 
-;; This default value ':formals will generate a list of options with
-;; the same value. This violates the constraint that options should be
-;; distinctive. But that's alright, since we never expect option-fix's logic
-;; formula to ever get used. Proved guards ensure it.
-(define function-option-name-fix ((option-name function-option-name-p))
-  :returns (fixed-option-name function-option-name-p)
-  :short "Fixing function for option."
-  (mbe :logic (if (function-option-name-p option-name) option-name ':formals)
-       :exec option-name))
+  (deffixtype argument-syntax
+    :pred  argument-syntax-p
+    :fix   argument-syntax-fix
+    :equiv argument-syntax-equiv
+    :define t
+    :forward t
+    :topic argument-syntax-p)
 
-(define function-option-name-lst-p ((option-lst t))
-  :returns (syntax-good? booleanp)
-  :short "Recoginizer for option-lst."
-  (b* (((if (atom option-lst)) (equal option-lst nil))
-       ((cons first rest) option-lst))
-    (and (function-option-name-p first)
-         (function-option-name-lst-p rest))))
 
-(define function-option-name-lst-fix ((option-lst function-option-name-lst-p))
-  :returns (fixed-option-lst function-option-name-lst-p
-                             :hints (("Goal" :in-theory (enable function-option-name-lst-p))))
-  :short "Fixing function for option-name-lst."
-  :verify-guards nil
-  (mbe :logic (if (atom option-lst)
-                  nil
-                (cons (function-option-name-fix (car option-lst))
-                      (function-option-name-lst-fix (cdr option-lst))))
-       :exec option-lst))
-(verify-guards function-option-name-lst-fix
-  :hints (("Goal" :in-theory (enable function-option-name-fix
-                                     function-option-name-lst-fix
-                                     function-option-name-p function-option-name-lst-p))))
+  (define argument-lst-syntax-fix ((term argument-lst-syntax-p))
+    :short "Fixing function for argument-lst-syntax."
+    :returns (fixed-term argument-lst-syntax-p
+                         :hints (("Goal"
+                                  :in-theory (enable argument-lst-syntax-p))))
+    :verify-guards nil
+    (mbe :logic (if (consp term)
+                    (cons (argument-syntax-fix (car term))
+                          (argument-lst-syntax-fix (cdr term)))
+                  nil)
+         :exec term))
+  (verify-guards argument-lst-syntax-fix
+    :hints (("Goal"
+             :in-theory (enable argument-lst-syntax-fix argument-syntax-fix argument-lst-syntax-p))))
 
-;; The conditions in eval-type should go along with *function-options*
-(define eval-function-option-type ((option-type function-option-type-p) (term t))
-  :returns (type-correct? booleanp)
-  :short "Evaluating types for function option body."
-  (b* ((option-type (function-option-type-fix option-type)))
+  (defthm argument-lst-syntax-fix-idempotent-lemma
+    (equal (argument-lst-syntax-fix (argument-lst-syntax-fix x))
+           (argument-lst-syntax-fix x))
+    :hints (("Goal" :in-theory (enable argument-lst-syntax-fix argument-syntax-fix))))
+
+  (deffixtype argument-lst-syntax
+    :pred  argument-lst-syntax-p
+    :fix   argument-lst-syntax-fix
+    :equiv argument-lst-syntax-equiv
+    :define t
+    :forward t
+    :topic argument-lst-syntax-p)
+
+  (defconst *function-options*
+    '((:formals . argument-lst-syntax-p)
+      (:returns . argument-lst-syntax-p)
+      (:level . qnatp)
+      (:guard . hypothesis-syntax-p)
+      (:more-returns . hypothesis-lst-syntax-p)))
+
+  (defconst *function-option-names*
+    (strip-cars *function-options*))
+
+  (defconst *function-option-types*
+    (remove-duplicates-equal (strip-cdrs *function-options*)))
+
+  (define function-option-type-p ((option-type t))
+    :returns (syntax-good? booleanp)
+    :short "Recoginizer for function-option-type."
+    (if (member-equal option-type *function-option-types*) t nil))
+
+  (define function-option-type-fix ((option-type function-option-type-p))
+    :returns (fixed-option-type function-option-type-p
+                                :hints (("Goal" :in-theory (enable
+                                                            function-option-type-p ))))
+    :short "Fixing function for function-option-type."
+    (mbe :logic (if (function-option-type-p option-type) option-type 'qnatp)
+         :exec option-type))
+
+  (define function-option-name-p ((option-name t))
+    :returns (syntax-good? booleanp)
+    :short "Recoginizer for an function-option-name."
+    (if (member-equal option-name *function-option-names*) t nil))
+
+  ;; This default value ':formals will generate a list of options with
+  ;; the same value. This violates the constraint that options should be
+  ;; distinctive. But that's alright, since we never expect option-fix's logic
+  ;; formula to ever get used. Proved guards ensure it.
+  (define function-option-name-fix ((option-name function-option-name-p))
+    :returns (fixed-option-name function-option-name-p)
+    :short "Fixing function for option."
+    (mbe :logic (if (function-option-name-p option-name) option-name ':formals)
+         :exec option-name))
+
+  (define function-option-name-lst-p ((option-lst t))
+    :returns (syntax-good? booleanp)
+    :short "Recoginizer for option-lst."
+    (b* (((if (atom option-lst)) (equal option-lst nil))
+         ((cons first rest) option-lst))
+      (and (function-option-name-p first)
+           (function-option-name-lst-p rest))))
+
+  (define function-option-name-lst-fix ((option-lst function-option-name-lst-p))
+    :returns (fixed-option-lst function-option-name-lst-p
+                               :hints (("Goal" :in-theory (enable function-option-name-lst-p))))
+    :short "Fixing function for option-name-lst."
+    :verify-guards nil
+    (mbe :logic (if (atom option-lst)
+                    nil
+                  (cons (function-option-name-fix (car option-lst))
+                        (function-option-name-lst-fix (cdr option-lst))))
+         :exec option-lst))
+  (verify-guards function-option-name-lst-fix
+    :hints (("Goal" :in-theory (enable function-option-name-fix
+                                       function-option-name-lst-fix
+                                       function-option-name-p function-option-name-lst-p))))
+
+  ;; The conditions in eval-type should go along with *function-options*
+  (define eval-function-option-type ((option-type function-option-type-p) (term t))
+    :returns (type-correct? booleanp)
+    :short "Evaluating types for function option body."
+    (b* ((option-type (function-option-type-fix option-type)))
+      (case option-type
+        (argument-lst-syntax-p (argument-lst-syntax-p term))
+        (qnatp (qnatp term))
+        (hypothesis-syntax-p (hypothesis-syntax-p term))
+        (t (hypothesis-lst-syntax-p term)))))
+
+  (define function-option-syntax-p ((term t) (used function-option-name-lst-p))
+    :returns (mv (syntax-good? booleanp)
+                 (used? function-option-name-lst-p
+                        :hints (("Goal" :in-theory (enable function-option-name-lst-p function-option-name-p)))))
+    :short "Recoginizer for function-option-syntax."
+    :verify-guards nil
+    (b* ((used (function-option-name-lst-fix used))
+         ((if (equal term nil)) (mv t used))
+         ((unless (and (true-listp term) (car term) (cadr term))) (mv nil used))
+         ((cons option body-lst) term)
+         ((unless (function-option-name-p option)) (mv nil used))
+         (option-type (cdr (assoc-equal option *function-options*))))
+      (mv (and (not (member-equal option used))
+               (eval-function-option-type option-type (car body-lst)))
+          (cons option used))))
+  (verify-guards function-option-syntax-p
+    :guard-debug t
+    :hints (("Goal" :in-theory (enable function-option-syntax-p function-option-name-p
+                                       eval-function-option-type function-option-name-lst-p))))
+
+  ;; (define exist-odd-lst ((key symbolp) (lst t))
+  ;;   :returns (exist? booleanp)
+  ;;   :short "Test if key exist in lst on the odd positions (with position staring
+  ;; from 1)"
+  ;;   :measure (len lst)
+  ;;   :hints (("Goal" :in-theory (enable true-list-fix)))
+  ;;   :verify-guards nil
+  ;;   (b* ((key (symbol-fix key))
+  ;;        ((if (equal lst nil)) nil)
+  ;;        ((unless (and (true-listp lst) (>= (len lst) 2))) nil)
+  ;;        ((list* first & rest) lst)
+  ;;        ((if (equal first key)) t))
+  ;;     (exist-odd-lst key rest)))
+  ;; (verify-guards exist-odd-lst
+  ;;   :hints (("Goal" :in-theory (enable true-list-fix))))
+
+  (define function-option-lst-syntax-p-helper ((term t) (used function-option-name-lst-p))
+    :returns (syntax-good? booleanp)
+    :short "Helper for function-option-lst-syntax-p."
+    (b* (((if (atom term)) (equal term nil))
+         ((unless (and (true-listp term) (>= (len term) 2))) nil)
+         ((list* first second rest) term)
+         ((mv res new-used) (function-option-syntax-p (list first second) used)))
+      (and res (function-option-lst-syntax-p-helper rest new-used)))
+    ///
+    (defthm function-option-lst-syntax-p-constraint
+      (implies (and (function-option-lst-syntax-p-helper fun-opt-lst nil)
+                    (consp fun-opt-lst))
+               (or (equal (car fun-opt-lst) ':formals)
+                   (equal (car fun-opt-lst) ':returns)
+                   (equal (car fun-opt-lst) ':level)
+                   (equal (car fun-opt-lst) ':guard)
+                   (equal (car fun-opt-lst) ':more-returns)))
+      :hints (("Goal"
+               :in-theory (enable eval-function-option-type
+                                  function-option-syntax-p
+                                  function-option-name-p))))
+
+    (defthm function-option-lst-syntax-p-of-option
+      (implies
+       (and (consp (cdr fun-opt-lst))
+            (function-option-lst-syntax-p-helper fun-opt-lst nil)
+            (consp fun-opt-lst))
+       (and (implies (equal (car fun-opt-lst) ':formals)
+                     (argument-lst-syntax-p (cadr fun-opt-lst)))
+            (implies (equal (car fun-opt-lst) ':returns)
+                     (argument-lst-syntax-p (cadr fun-opt-lst)))
+            (implies (equal (car fun-opt-lst) ':level)
+                     (qnatp (cadr fun-opt-lst)))
+            (implies (equal (car fun-opt-lst) ':guard)
+                     (hypothesis-syntax-p (cadr fun-opt-lst)))
+            (implies (equal (car fun-opt-lst) ':more-returns)
+                     (hypothesis-lst-syntax-p (cadr fun-opt-lst)))))
+      :hints (("Goal"
+               :in-theory (enable function-option-syntax-p
+                                  eval-function-option-type))))
+
+    (skip-proofs
+     (defthm function-option-lst-syntax-preserve
+       (implies (and (function-option-lst-syntax-p-helper term nil)
+                     (consp term))
+                (function-option-lst-syntax-p-helper (cddr term)
+                                                     nil))
+       :hints (("Goal"
+                :in-theory (enable function-option-syntax-p))))
+     ))
+
+  (define function-option-lst-syntax-p ((term t))
+    :returns (syntax-good? booleanp)
+    :short "Recogizer for function-option-lst-syntax"
+    (function-option-lst-syntax-p-helper term nil))
+
+  (define function-option-lst-syntax-fix ((term function-option-lst-syntax-p))
+    :returns (fixed-term function-option-lst-syntax-p)
+    :short "Recogizer for function-option-lst-syntax"
+    (mbe :logic (if (function-option-lst-syntax-p term) term nil)
+         :exec term))
+
+  (defthm function-option-lst-syntax-fix-idempotent-lemma
+    (equal (function-option-lst-syntax-fix (function-option-lst-syntax-fix x))
+           (function-option-lst-syntax-fix x))
+    :hints (("Goal" :in-theory (enable function-option-lst-syntax-fix))))
+
+  (deffixtype function-option-lst-syntax
+    :pred  function-option-lst-syntax-p
+    :fix   function-option-lst-syntax-fix
+    :equiv function-option-lst-syntax-equiv
+    :define t
+    :forward t
+    :topic function-option-lst-syntax-p)
+
+  (define function-syntax-p ((term t))
+    :returns (syntax-good? booleanp)
+    :short "Recognizer for function-syntax."
+    (b* (((unless (true-listp term)) nil)
+         ((unless (consp term)) t)
+         ((cons fname function-options) term))
+      ;; It's probably possible to check existence of function?
+      ;; Currently not doing such check, since it will require passing state.
+      (and (symbolp fname)
+           (function-option-lst-syntax-p function-options))))
+
+  (define function-syntax-fix ((term function-syntax-p))
+    :returns (fixed-term function-syntax-p)
+    :short "Fixing function for function-syntax-p"
+    (mbe :logic (if (function-syntax-p term) term nil)
+         :exec term))
+
+  (defthm function-syntax-fix-idempotent-lemma
+    (equal (function-syntax-fix (function-syntax-fix x))
+           (function-syntax-fix x))
+    :hints (("Goal" :in-theory (enable function-syntax-fix))))
+
+  (deffixtype function-syntax
+    :pred  function-syntax-p
+    :fix   function-syntax-fix
+    :equiv function-syntax-equiv
+    :define t
+    :forward t
+    :topic function-syntax-p)
+
+  (define function-lst-syntax-p ((term t))
+    :returns (syntax-good? booleanp)
+    :short "Recognizer for function-lst-syntax"
+    (b* (((if (atom term)) (equal term nil))
+         ((cons first rest) term))
+      (and (function-syntax-p first)
+           (function-lst-syntax-p rest))))
+
+  (define function-lst-syntax-fix ((term function-lst-syntax-p))
+    :returns (fixed-term function-lst-syntax-p
+                         :hints (("Goal" :in-theory (enable
+                                                     function-lst-syntax-p))))
+    :short "Fixing function for function-lst-syntax-fix"
+    :verify-guards nil
+    (mbe :logic (if (consp term)
+                    (cons (function-syntax-fix (car term))
+                          (function-lst-syntax-fix (cdr term)))
+                  nil)
+         :exec term))
+  (verify-guards function-lst-syntax-fix
+    :hints (("Goal" :in-theory (enable function-lst-syntax-fix
+                                       function-syntax-fix function-lst-syntax-p function-syntax-p))))
+
+  (defthm function-lst-syntax-fix-idempotent-lemma
+    (equal (function-lst-syntax-fix (function-lst-syntax-fix x))
+           (function-lst-syntax-fix x))
+    :hints (("Goal" :in-theory (enable function-lst-syntax-fix))))
+
+  (deffixtype function-lst-syntax
+    :pred  function-lst-syntax-p
+    :fix   function-lst-syntax-fix
+    :equiv function-lst-syntax-equiv
+    :define t
+    :forward t
+    :topic function-lst-syntax-p)
+
+
+  (define smt-solver-params-p ((term t))
+    :returns (syntax-good? booleanp)
+    :short "Recognizer for smt-solver-params."
+    (true-listp term))
+
+  (define smt-solver-params-fix ((term smt-solver-params-p))
+    :returns (fixed-term smt-solver-params-p
+                         :hints (("Goal" :in-theory (enable smt-solver-params-p))))
+    :short "Fixing function for smt-solver-params."
+    (mbe :logic (if (smt-solver-params-p term) term (true-list-fix term))
+         :exec term))
+
+  (defconst *cnf-options*
+    '(:interface-dir :SMT-files-dir :SMT-module
+                     :SMT-class :SMT-cmd :file-format))
+
+  (define cnf-option-p ((option t))
+    :returns (syntax-good? booleanp)
+    :short "Recoginizer for cnf-option."
+    (if (member-equal option *cnf-options*) t nil))
+
+  (define cnf-option-fix ((option cnf-option-p))
+    :returns (fixed-cnf-option cnf-option-p)
+    :short "Fixing function for cnf-option."
+    (mbe :logic (if (cnf-option-p option) option ':interface-dir)
+         :exec option))
+
+  (define cnf-option-lst-p ((option-lst t))
+    :returns (syntax-good? booleanp)
+    :short "Recoginizer for cnf-option-lst."
+    (b* (((if (atom option-lst)) (equal option-lst nil))
+         ((cons first rest) option-lst))
+      (and (cnf-option-p first)
+           (cnf-option-lst-p rest))))
+
+  (define cnf-option-lst-fix ((option-lst cnf-option-lst-p))
+    :returns (fixed-option-lst cnf-option-lst-p
+                               :hints (("Goal" :in-theory (enable cnf-option-lst-p))))
+    :short "Fixing function for cnf-option-lst."
+    :verify-guards nil
+    (mbe :logic (if (atom option-lst)
+                    nil
+                  (cons (cnf-option-fix (car option-lst))
+                        (cnf-option-lst-fix (cdr option-lst))))
+         :exec option-lst))
+  (verify-guards cnf-option-lst-fix
+    :hints (("Goal" :in-theory (enable cnf-option-fix
+                                       cnf-option-lst-fix
+                                       cnf-option-p cnf-option-lst-p))))
+
+
+  (define smt-solver-single-cnf-p ((term t) (used cnf-option-lst-p))
+    :returns (mv (syntax-good? booleanp)
+                 (new-used cnf-option-lst-p
+                           :hints (("Goal" :in-theory (enable cnf-option-lst-p cnf-option-p)))))
+    :short "Recognizer for smt-solver-single-cnf."
+    (b* ((used (cnf-option-lst-fix used))
+         ((if (equal term nil)) (mv t used))
+         ((unless (and (true-listp term) (car term) (cadr term))) (mv nil used))
+         ((cons option body-lst) term)
+         ((unless (cnf-option-p option)) (mv nil used)))
+      (mv (and (not (member-equal option used))
+               (qstringp (car body-lst)))
+          (cons option used))))
+
+  (defthm member-equal-preserve
+    (implies (not (member-equal x (cons a lst)))
+             (not (member-equal x lst))))
+
+  (define smt-solver-cnf-p-helper ((term t) (used cnf-option-lst-p))
+    :returns (syntax-good? booleanp)
+    :short "Helper function for smt-solver-cnf-p."
+    (b* (((if (atom term)) (equal term nil))
+         ((unless (and (true-listp term) (>= (len term) 2))) nil)
+         ((list* first second rest) term)
+         ((mv res new-used) (smt-solver-single-cnf-p (list first second) used)))
+      (and res (smt-solver-cnf-p-helper rest new-used)))
+    ///
+    (defthm crock-true-listp
+      (implies (smt-solver-cnf-p-helper term nil)
+               (true-listp term)))
+
+    (defthm stringp-of-cadr
+      (implies (and (smt-solver-cnf-p-helper content nil)
+                    (consp content))
+               (stringp (cadadr content)))
+      :hints (("Goal"
+               :in-theory (enable smt-solver-single-cnf-p cnf-option-p
+                                  qstringp))))
+    (skip-proofs
+     (defthm cddr-preserve
+       (implies (and (smt-solver-cnf-p-helper content nil)
+                     (consp content))
+                (smt-solver-cnf-p-helper (cddr content)
+                                         nil))
+       :hints (("Goal"
+                :in-theory (enable smt-solver-cnf-p-helper smt-solver-single-cnf-p member-equal)
+                ;; :use ((:instance member-equal-preserve
+                ;;                  (x )
+                ;;                  (a )
+                ;;                  (lst )))
+                ))))
+    )
+
+  (define smt-solver-cnf-p ((term t))
+    :returns (syntax-good? booleanp)
+    :short "Recognizer for smt-solver-cnf."
+    (smt-solver-cnf-p-helper term nil))
+
+  (define smt-solver-cnf-fix ((term smt-solver-cnf-p))
+    :returns (fixed-smt-cnf smt-solver-cnf-p)
+    :short "Fixing function for smt-solver-cnf."
+    (mbe :logic (if (smt-solver-cnf-p term) term nil)
+         :exec term))
+
+  (defthm smt-solver-cnf-fix-idempotent-lemma
+    (equal (smt-solver-cnf-fix (smt-solver-cnf-fix x))
+           (smt-solver-cnf-fix x))
+    :hints (("Goal" :in-theory (enable smt-solver-cnf-fix))))
+
+  (deffixtype smt-solver-cnf
+    :pred  smt-solver-cnf-p
+    :fix   smt-solver-cnf-fix
+    :equiv smt-solver-cnf-equiv
+    :define t
+    :forward t
+    :topic smt-solver-cnf-p)
+
+  (defconst *smtlink-options*
+    '((:functions . function-lst-syntax-p)
+      (:hypothesis . hypothesis-lst-syntax-p)
+      (:main-hint . hints-syntax-p)
+      (:int-to-rat . qbooleanp)
+      (:smt-fname . qstringp)
+      (:rm-file . qbooleanp)
+      (:smt-solver-params . smt-solver-params-p)
+      (:smt-solver-cnf . smt-solver-cnf-p)))
+
+  (defconst *smtlink-option-names*
+    (strip-cars *smtlink-options*))
+
+  (defconst *smtlink-option-types*
+    (remove-duplicates-equal (strip-cdrs *smtlink-options*)))
+
+  (define smtlink-option-type-p ((option-type t))
+    :returns (syntax-good? booleanp)
+    :short "Recoginizer for smtlink-option-type."
+    (if (member-equal option-type *smtlink-option-types*) t nil))
+
+  (define smtlink-option-type-fix ((opttype smtlink-option-type-p))
+    :returns (fixed-opttype smtlink-option-type-p
+                            :hints (("Goal" :in-theory (enable
+                                                        smtlink-option-type-p))))
+    :short "Fixing function for smtlink-option-type."
+    (mbe :logic (if (smtlink-option-type-p opttype) opttype 'function-lst-syntax-p)
+         :exec opttype))
+
+  (define smtlink-option-name-p ((option-name t))
+    :returns (syntax-good? booleanp)
+    :short "Recoginizer for an smtlink-option-name."
+    (if (member-equal option-name *smtlink-option-names*) t nil))
+
+  (define smtlink-option-name-fix ((option smtlink-option-name-p))
+    :returns (fixed-smtlink-option-name smtlink-option-name-p)
+    :short "Fixing function for smtlink-option-name."
+    (mbe :logic (if (smtlink-option-name-p option) option ':functions)
+         :exec option))
+
+  (define smtlink-option-name-lst-p ((option-lst t))
+    :returns (syntax-good? booleanp)
+    :short "Recoginizer for smtlink-option-name-lst."
+    (b* (((if (atom option-lst)) (equal option-lst nil))
+         ((cons first rest) option-lst))
+      (and (smtlink-option-name-p first)
+           (smtlink-option-name-lst-p rest))))
+
+  (define smtlink-option-name-lst-fix ((option-lst smtlink-option-name-lst-p))
+    :returns (fixed-option-name-lst smtlink-option-name-lst-p
+                                    :hints (("Goal" :in-theory (enable smtlink-option-name-lst-p))))
+    :short "Fixing function for option-name-lst."
+    :verify-guards nil
+    (mbe :logic (if (atom option-lst)
+                    nil
+                  (cons (smtlink-option-name-fix (car option-lst))
+                        (smtlink-option-name-lst-fix (cdr option-lst))))
+         :exec option-lst))
+  (verify-guards smtlink-option-name-lst-fix
+    :hints (("Goal" :in-theory (enable smtlink-option-name-fix
+                                       smtlink-option-name-lst-fix
+                                       smtlink-option-name-p smtlink-option-name-lst-p))))
+
+  (define eval-smtlink-option-type ((option-type smtlink-option-type-p) (term t))
+    :returns (type-correct? booleanp)
+    :short "Evaluating types for smtlink option body."
     (case option-type
-      (argument-lst-syntax-p (argument-lst-syntax-p term))
-      (qnatp (qnatp term))
-      (t (hypothesis-lst-syntax-p term)))))
+      (function-lst-syntax-p (function-lst-syntax-p term))
+      (hypothesis-lst-syntax-p (hypothesis-lst-syntax-p term))
+      (hints-syntax-p (hints-syntax-p term))
+      (qbooleanp (qbooleanp term))
+      (qstringp (qstringp term))
+      (smt-solver-params-p (smt-solver-params-p term))
+      (t (smt-solver-cnf-p term))))
 
-(define function-option-syntax-p ((term t) (used function-option-name-lst-p))
-  :returns (mv (syntax-good? booleanp)
-               (used? function-option-name-lst-p
-                      :hints (("Goal" :in-theory (enable function-option-name-lst-p function-option-name-p)))))
-  :short "Recoginizer for function-option-syntax."
-  :verify-guards nil
-  (b* ((used (function-option-name-lst-fix used))
-       ((if (equal term nil)) (mv t used))
-       ((unless (and (true-listp term) (equal (len term) 2))) (mv nil used))
-       ((cons option body-lst) term)
-       ((unless (function-option-name-p option)) (mv nil used))
-       (option-type (cdr (assoc-equal option *function-options*))))
-    (mv (and (not (member-equal option used))
-             (eval-function-option-type option-type (car body-lst)))
-        (cons option used))))
-(verify-guards function-option-syntax-p
-  :guard-debug t
-  :hints (("Goal" :in-theory (enable function-option-syntax-p function-option-name-p
-                                     eval-function-option-type function-option-name-lst-p))))
+  (define smtlink-option-syntax-p ((term t) (used smtlink-option-name-lst-p))
+    :returns (mv (syntax-good? booleanp)
+                 (used? smtlink-option-name-lst-p
+                        :hints (("Goal" :in-theory (enable smtlink-option-name-lst-p smtlink-option-name-p)))))
+    :short "Recoginizer for smtlink-option-syntax."
+    :verify-guards nil
+    (b* ((used (smtlink-option-name-lst-fix used))
+         ((if (equal term nil)) (mv t used))
+         ((unless (and (true-listp term) (car term) (cadr term))) (mv nil used))
+         ((cons option body-lst) term)
+         ((unless (smtlink-option-name-p option)) (mv nil used))
+         (option-type (cdr (assoc-equal option *smtlink-options*))))
+      (mv (and (not (member-equal option used))
+               (eval-smtlink-option-type option-type (car body-lst)))
+          (cons option used))))
+  (verify-guards smtlink-option-syntax-p
+    :guard-debug t
+    :hints (("Goal" :in-theory (enable smtlink-option-syntax-p smtlink-option-name-p
+                                       eval-smtlink-option-type smtlink-option-name-lst-p))))
 
-(define function-option-lst-syntax-p-helper ((term t) (used function-option-name-lst-p))
-  :returns (syntax-good? booleanp)
-  :short "Helper for function-option-lst-syntax-p."
-  (b* (((if (atom term)) (equal term nil))
-       ((unless (and (true-listp term) (>= (len term) 2))) nil)
-       ((list* first second rest) term)
-       ((mv res new-used) (function-option-syntax-p (list first second) used)))
-    (and res (function-option-lst-syntax-p-helper rest new-used)))
-  ///
-  (skip-proofs
-  (defthm function-option-lst-syntax-preserve
-    (implies (and (function-option-lst-syntax-p-helper term nil)
-                  (consp term))
-             (function-option-lst-syntax-p-helper (cddr term)
-                                                  nil))))
+  (define smtlink-hint-syntax-p-helper ((term t) (used smtlink-option-name-lst-p))
+    :returns (syntax-good? booleanp)
+    :short "Helper function for smtlink-hint-syntax-p."
+    (b* (((if (atom term)) (equal term nil))
+         ((unless (and (true-listp term) (>= (len term) 2))) nil)
+         ((list* first second rest) term)
+         ((mv res new-used) (smtlink-option-syntax-p (list first second) used)))
+      (and res (smtlink-hint-syntax-p-helper rest new-used)))
+    ///
+    (defthm function-lst-syntax-p-constraint
+      (implies (and (smtlink-hint-syntax-p-helper user-hint nil)
+                    (consp user-hint)
+                    (consp (cdr user-hint)))
+               (or (equal (car user-hint) ':functions)
+                   (equal (car user-hint) ':hypothesis)
+                   (equal (car user-hint) ':main-hint)
+                   (equal (car user-hint) ':int-to-rat)
+                   (equal (car user-hint) ':smt-fname)
+                   (equal (car user-hint) ':rm-file)
+                   (equal (car user-hint) ':smt-solver-params)
+                   (equal (car user-hint) ':smt-solver-cnf)))
+      :hints (("Goal"
+               :in-theory (enable eval-smtlink-option-type
+                                  smtlink-option-syntax-p
+                                  smtlink-option-name-p))))
 
-  (defthm function-option-lst-syntax-p-constraint
-    (implies (and (function-option-lst-syntax-p-helper fun-opt-lst nil)
-                  (consp fun-opt-lst))
-             (or (equal (car fun-opt-lst) ':formals)
-                 (equal (car fun-opt-lst) ':returns)
-                 (equal (car fun-opt-lst) ':level)
-                 (equal (car fun-opt-lst) ':guard)
-                 (equal (car fun-opt-lst) ':more-returns)))
+    (defthm function-lst-syntax-p-of-option
+      (implies
+       (and (consp (cdr user-hint))
+            (smtlink-hint-syntax-p-helper user-hint nil)
+            (consp user-hint))
+       (and (implies (equal (car user-hint) ':functions)
+                     (function-lst-syntax-p (cadr user-hint)))
+            (implies (equal (car user-hint) ':hypothesis)
+                     (hypothesis-lst-syntax-p (cadr user-hint)))
+            (implies (equal (car user-hint) ':main-hint)
+                     (hints-syntax-p (cadr user-hint)))
+            (implies (equal (car user-hint) ':int-to-rat)
+                     (qbooleanp (cadr user-hint)))
+            (implies (equal (car user-hint) ':smt-fname)
+                     (qstringp (cadr user-hint)))
+            (implies (equal (car user-hint) ':rm-file)
+                     (qbooleanp (cadr user-hint)))
+            (implies (equal (car user-hint) ':smt-solver-params)
+                     (smt-solver-params-p (cadr user-hint)))
+            (implies (equal (car user-hint) ':smt-solver-cnf)
+                     (smt-solver-cnf-p (cadr user-hint)))))
+      :hints (("Goal"
+               :in-theory (enable smtlink-option-syntax-p
+                                  eval-smtlink-option-type))))
+
+    (skip-proofs
+     (defthm smtlink-hint-syntax-preserve
+       (implies (and (smtlink-hint-syntax-p-helper term nil)
+                     (consp term))
+                (smtlink-hint-syntax-p-helper (cddr term)
+                                              nil))))
+    )
+
+  (define smtlink-hint-syntax-p ((term t))
+    :returns (syntax-good? booleanp)
+    :short "Recognizer for smtlink-hint-syntax."
+    (smtlink-hint-syntax-p-helper term nil))
+
+  ;; Strange fixing function.
+  (define smtlink-hint-syntax-fix ((term smtlink-hint-syntax-p))
+    :short "Fixing function for smtlink-hint-syntax."
+    :returns (fixed-smtlink-hint-syntax smtlink-hint-syntax-p)
+    (mbe :logic (if (smtlink-hint-syntax-p term) term nil)
+         :exec term))
+
+  ;; -------------------------------------------------------------------------
+  ;; (local (in-theory (enable pseudo-termp)))
+
+  ;; (defthm symbolp-is-pseudo-termp-crock
+  ;;   (implies (symbolp x) (pseudo-termp x)))
+
+  (define make-merge-formals-helper ((content argument-lst-syntax-p) (smt-func func-p))
+    :returns (func func-p)
+    :short "Adding user defined formals to overwrite what's already in smt-func."
+    :measure (len content)
+    :hints (("Goal" :in-theory (enable argument-lst-syntax-fix)))
+    :verify-guards nil
+    (b* ((content (argument-lst-syntax-fix content))
+         (smt-func (func-fix smt-func))
+         ((func f) smt-func)
+         ((unless (consp content)) smt-func)
+         ((cons first rest) content)
+         ((list* argname type & hints) first)
+         (new-formals (cons (make-decl :name argname
+                                       :type (make-hint-pair :thm type
+                                                             :hints hints))
+                            f.formals))
+         (new-func (change-func f :formals new-formals)))
+      (make-merge-formals-helper rest new-func)))
+
+  (verify-guards make-merge-formals-helper
+    :hints (("Goal" :in-theory (enable argument-lst-syntax-fix
+                                       argument-lst-syntax-p
+                                       argument-syntax-fix
+                                       argument-syntax-p
+                                       smt-typep
+                                       hints-syntax-p))))
+
+  (define remove-duplicate-from-decl-list ((decls decl-listp) (seen symbol-listp))
+    :returns (simple-decls decl-listp)
+    :short "Remove shadowed decls from decl-list"
+    :measure (len decls)
+    (b* ((decls (decl-list-fix decls))
+         ((unless (consp decls)) nil)
+         ((cons first rest) decls)
+         ((decl d) first)
+         (seen? (member-equal d.name seen))
+         ((if seen?) (remove-duplicate-from-decl-list rest seen)))
+      (cons first (remove-duplicate-from-decl-list rest (cons d.name seen)))))
+
+  (define make-merge-formals ((content argument-lst-syntax-p) (smt-func func-p))
+    :returns (func func-p)
+    :short "Adding user defined formals to overwrite what's already in smt-func."
+    (b* ((new-func (make-merge-formals-helper content smt-func))
+         ((func f) new-func))
+      (change-func f :formals (remove-duplicate-from-decl-list f.formals nil))))
+
+  (define make-merge-returns-helper ((content argument-lst-syntax-p) (smt-func func-p))
+    :returns (func func-p)
+    :short "Adding user defined returns to overwrite what's already in smt-func."
+    :measure (len content)
+    :hints (("Goal" :in-theory (enable argument-lst-syntax-fix)))
+    :verify-guards nil
+    (b* ((content (argument-lst-syntax-fix content))
+         (smt-func (func-fix smt-func))
+         ((func f) smt-func)
+         ((unless (consp content)) smt-func)
+         ((cons first rest) content)
+         ((cons argname (cons type (cons & hints))) first)
+         (new-formals (cons (make-decl :name argname
+                                       :type (make-hint-pair :thm type
+                                                             :hints hints))
+                            f.formals))
+         (new-func (change-func f :returns new-formals)))
+      (make-merge-returns-helper rest new-func)))
+
+  (verify-guards make-merge-returns-helper
+    :hints (("Goal" :in-theory (enable argument-lst-syntax-fix
+                                       argument-lst-syntax-p
+                                       argument-syntax-p
+                                       argument-syntax-fix
+                                       hints-syntax-p
+                                       smt-typep
+                                       ))))
+
+  (define make-merge-returns ((content argument-lst-syntax-p) (smt-func func-p))
+    :returns (func func-p)
+    :short "Adding user defined returns to overwrite what's already in smt-func."
+    (b* ((new-func (make-merge-returns-helper content smt-func))
+         ((func f) new-func))
+      (change-func f :formals (remove-duplicate-from-decl-list f.formals nil))))
+
+  (define make-merge-guard ((content hypothesis-syntax-p) (smt-func func-p))
+    :returns (func func-p)
+    :short "Adding user defined guard to smt-func."
+    :verify-guards nil
+    (b* ((content (hypothesis-syntax-fix content))
+         (smt-func (func-fix smt-func))
+         ((cons thm (cons & hints-lst)) content)
+         (hints (car hints-lst))
+         (new-guard (make-hint-pair :thm thm :hints hints)))
+      (change-func smt-func :guard new-guard)))
+
+  (verify-guards make-merge-guard
     :hints (("Goal"
-             :in-theory (enable eval-function-option-type
-                                function-option-syntax-p
-                                function-option-name-p))))
+             :in-theory (enable hypothesis-syntax-fix hypothesis-syntax-p))))
 
-  (defthm function-option-lst-syntax-p-of-option
-    (implies
-     (and (consp (cdr fun-opt-lst))
-          (function-option-lst-syntax-p-helper fun-opt-lst nil)
-          (consp fun-opt-lst))
-     (and (implies (equal (car fun-opt-lst) ':formals)
-                   (argument-lst-syntax-p (cadr fun-opt-lst)))
-          (implies (equal (car fun-opt-lst) ':returns)
-                   (argument-lst-syntax-p (cadr fun-opt-lst)))
-          (implies (equal (car fun-opt-lst) ':level)
-                   (qnatp (cadr fun-opt-lst)))
-          (implies (equal (car fun-opt-lst) ':guard)
-                   (hypothesis-lst-syntax-p (cadr fun-opt-lst)))
-          (implies (equal (car fun-opt-lst) ':more-returns)
-                   (hypothesis-lst-syntax-p (cadr fun-opt-lst)))))
+
+  (define make-merge-more-returns ((content hypothesis-lst-syntax-p)
+                                   (smt-func func-p))
+    :returns (func func-p)
+    :short "Adding user-defined more-return theorems."
+    :measure (len content)
+    :hints (("Goal" :in-theory (enable hypothesis-lst-syntax-fix)))
+    :verify-guards nil
+    (b* ((content (hypothesis-lst-syntax-fix content))
+         (smt-func (func-fix smt-func))
+         ((func f) smt-func)
+         ((unless (consp content)) smt-func)
+         ((cons first rest) content)
+         ((cons thm (cons & hints-lst)) first)
+         (hints (car hints-lst))
+         (new-more-return (make-hint-pair :thm thm :hints hints))
+         (new-func (change-func smt-func
+                                :more-returns (cons new-more-return f.more-returns))))
+      (make-merge-more-returns rest new-func)))
+
+  (defthm cdr-of-hypothesis-lst-syntax-fix-crock
+    (hypothesis-lst-syntax-p (cdr (hypothesis-lst-syntax-fix content)))
     :hints (("Goal"
-             :in-theory (enable function-option-syntax-p
-                                eval-function-option-type))))
-  )
+             :in-theory (enable hypothesis-lst-syntax-fix))))
 
-(define function-option-lst-syntax-p ((term t))
-  :returns (syntax-good? booleanp)
-  :short "Recogizer for function-option-lst-syntax"
-  (function-option-lst-syntax-p-helper term nil))
+  (verify-guards make-merge-more-returns
+    :guard-debug t
+    :hints (("Goal" :in-theory (enable hypothesis-lst-syntax-p
+                                       hypothesis-lst-syntax-fix
+                                       hypothesis-syntax-p
+                                       hypothesis-syntax-fix))))
 
-(define function-option-lst-syntax-fix ((term function-option-lst-syntax-p))
-  :returns (fixed-term function-option-lst-syntax-p)
-  :short "Recogizer for function-option-lst-syntax"
-  (mbe :logic (if (function-option-lst-syntax-p term) term nil)
-       :exec term))
-
-(defthm function-option-lst-syntax-fix-idempotent-lemma
-  (equal (function-option-lst-syntax-fix (function-option-lst-syntax-fix x))
-         (function-option-lst-syntax-fix x))
-  :hints (("Goal" :in-theory (enable function-option-lst-syntax-fix))))
-
-(deffixtype function-option-lst-syntax
-  :pred  function-option-lst-syntax-p
-  :fix   function-option-lst-syntax-fix
-  :equiv function-option-lst-syntax-equiv
-  :define t
-  :forward t
-  :topic function-option-lst-syntax-p)
-
-(define function-syntax-p ((term t))
-  :returns (syntax-good? booleanp)
-  :short "Recognizer for function-syntax."
-  (b* (((unless (true-listp term)) nil)
-       ((unless (consp term)) t)
-       ((cons fname function-options) term))
-    ;; It's probably possible to check existence of function?
-    ;; Currently not doing such check, since it will require passing state.
-    (and (symbolp fname)
-         (function-option-lst-syntax-p function-options))))
-
-(define function-syntax-fix ((term function-syntax-p))
-  :returns (fixed-term function-syntax-p)
-  :short "Fixing function for function-syntax-p"
-  (mbe :logic (if (function-syntax-p term) term nil)
-       :exec term))
-
-(defthm function-syntax-fix-idempotent-lemma
-  (equal (function-syntax-fix (function-syntax-fix x))
-         (function-syntax-fix x))
-  :hints (("Goal" :in-theory (enable function-syntax-fix))))
-
-(deffixtype function-syntax
-  :pred  function-syntax-p
-  :fix   function-syntax-fix
-  :equiv function-syntax-equiv
-  :define t
-  :forward t
-  :topic function-syntax-p)
-
-(define function-lst-syntax-p ((term t))
-  :returns (syntax-good? booleanp)
-  :short "Recognizer for function-lst-syntax"
-  (b* (((if (atom term)) (equal term nil))
-       ((cons first rest) term))
-    (and (function-syntax-p first)
-         (function-lst-syntax-p rest))))
-
-(define function-lst-syntax-fix ((term function-lst-syntax-p))
-  :returns (fixed-term function-lst-syntax-p
-                       :hints (("Goal" :in-theory (enable
-                                                   function-lst-syntax-p))))
-  :short "Fixing function for function-lst-syntax-fix"
-  :verify-guards nil
-  (mbe :logic (if (consp term)
-                  (cons (function-syntax-fix (car term))
-                        (function-lst-syntax-fix (cdr term)))
-                nil)
-       :exec term))
-(verify-guards function-lst-syntax-fix
-  :hints (("Goal" :in-theory (enable function-lst-syntax-fix
-  function-syntax-fix function-lst-syntax-p function-syntax-p))))
-
-(defthm function-lst-syntax-fix-idempotent-lemma
-  (equal (function-lst-syntax-fix (function-lst-syntax-fix x))
-         (function-lst-syntax-fix x))
-  :hints (("Goal" :in-theory (enable function-lst-syntax-fix))))
-
-(deffixtype function-lst-syntax
-  :pred  function-lst-syntax-p
-  :fix   function-lst-syntax-fix
-  :equiv function-lst-syntax-equiv
-  :define t
-  :forward t
-  :topic function-lst-syntax-p)
-
-
-(define smt-solver-params-p ((term t))
-  :returns (syntax-good? booleanp)
-  :short "Recognizer for smt-solver-params."
-  (true-listp term))
-
-(define smt-solver-params-fix ((term smt-solver-params-p))
-  :returns (fixed-term smt-solver-params-p
-                       :hints (("Goal" :in-theory (enable smt-solver-params-p))))
-  :short "Fixing function for smt-solver-params."
-  (mbe :logic (if (smt-solver-params-p term) term (true-list-fix term))
-       :exec term))
-
-(defconst *cnf-options*
-  '(:interface-dir :SMT-files-dir :SMT-module
-                   :SMT-class :SMT-cmd :file-format))
-
-(define cnf-option-p ((option t))
-  :returns (syntax-good? booleanp)
-  :short "Recoginizer for cnf-option."
-  (if (member-equal option *cnf-options*) t nil))
-
-(define cnf-option-fix ((option cnf-option-p))
-  :returns (fixed-cnf-option cnf-option-p)
-  :short "Fixing function for cnf-option."
-  (mbe :logic (if (cnf-option-p option) option ':interface-dir)
-       :exec option))
-
-(define cnf-option-lst-p ((option-lst t))
-  :returns (syntax-good? booleanp)
-  :short "Recoginizer for cnf-option-lst."
-  (b* (((if (atom option-lst)) (equal option-lst nil))
-       ((cons first rest) option-lst))
-    (and (cnf-option-p first)
-         (cnf-option-lst-p rest))))
-
-(define cnf-option-lst-fix ((option-lst cnf-option-lst-p))
-  :returns (fixed-option-lst cnf-option-lst-p
-                             :hints (("Goal" :in-theory (enable cnf-option-lst-p))))
-  :short "Fixing function for cnf-option-lst."
-  :verify-guards nil
-  (mbe :logic (if (atom option-lst)
-                  nil
-                (cons (cnf-option-fix (car option-lst))
-                      (cnf-option-lst-fix (cdr option-lst))))
-       :exec option-lst))
-(verify-guards cnf-option-lst-fix
-  :hints (("Goal" :in-theory (enable cnf-option-fix
-                                     cnf-option-lst-fix
-                                     cnf-option-p cnf-option-lst-p))))
-
-
-(define smt-solver-single-cnf-p ((term t) (used cnf-option-lst-p))
-  :returns (mv (syntax-good? booleanp)
-               (new-used cnf-option-lst-p
-                         :hints (("Goal" :in-theory (enable cnf-option-lst-p cnf-option-p)))))
-  :short "Recognizer for smt-solver-single-cnf."
-  (b* ((used (cnf-option-lst-fix used))
-       ((if (equal term nil)) (mv t used))
-       ((unless (and (true-listp term) (equal (len term) 2))) (mv nil used))
-       ((cons option body-lst) term)
-       ((unless (cnf-option-p option)) (mv nil used)))
-    (mv (and (not (member-equal option used))
-             (qstringp (car body-lst)))
-        (cons option used))))
-
-(defthm member-equal-preserve
-  (implies (not (member-equal x (cons a lst)))
-           (not (member-equal x lst))))
-
-(define smt-solver-cnf-p-helper ((term t) (used cnf-option-lst-p))
-  :returns (syntax-good? booleanp)
-  :short "Helper function for smt-solver-cnf-p."
-  (b* (((if (atom term)) (equal term nil))
-       ((unless (and (true-listp term) (>= (len term) 2))) nil)
-       ((list* first second rest) term)
-       ((mv res new-used) (smt-solver-single-cnf-p (list first second) used)))
-    (and res (smt-solver-cnf-p-helper rest new-used)))
-  ///
-  (defthm crock-true-listp
-    (implies (smt-solver-cnf-p-helper term nil)
-             (true-listp term)))
-
-  (defthm stringp-of-cadr
-    (implies (and (smt-solver-cnf-p-helper content nil)
-                  (consp content))
-             (stringp (cadadr content)))
+  ;; BOZO:
+  ;; This implementation is potentially slow because of the threading of smt-func
+  ;; all the way while at the same time updating it.
+  (define make-merge-function-option-lst ((fun-opt-lst function-option-lst-syntax-p)
+                                          (smt-func func-p))
+    :returns (func func-p)
+    :short "Add option information into func."
+    :measure (len fun-opt-lst)
+    :hints (("Goal" :in-theory (enable function-option-lst-syntax-fix)))
+    :verify-guards nil
+    (b* ((fun-opt-lst (function-option-lst-syntax-fix fun-opt-lst))
+         (smt-func (func-fix smt-func))
+         ((unless (consp fun-opt-lst)) smt-func)
+         ((cons option (cons content rest)) fun-opt-lst)
+         (new-func (case option
+                     (:formals (make-merge-formals content smt-func))
+                     (:returns (make-merge-returns content smt-func))
+                     (:level (change-func smt-func :expansion-depth (cadr content)))
+                     (:guard (make-merge-guard content smt-func))
+                     (:more-returns (make-merge-more-returns content smt-func)))))
+      (make-merge-function-option-lst rest new-func)))
+  (verify-guards make-merge-function-option-lst
     :hints (("Goal"
-             :in-theory (enable smt-solver-single-cnf-p cnf-option-p
-                                qstringp))))
-  (skip-proofs
-  (defthm cddr-preserve
-    (implies (and (smt-solver-cnf-p-helper content nil)
-                  (consp content))
-             (smt-solver-cnf-p-helper (cddr content)
-                                      nil))
+             :in-theory (enable function-option-lst-syntax-fix
+                                function-option-lst-syntax-p
+                                function-option-lst-syntax-p-helper
+                                hypothesis-lst-syntax-p
+                                qnatp)
+             :use ((:instance function-option-lst-syntax-p-of-option)
+                   (:instance function-option-lst-syntax-p-constraint)))))
+
+  (define make-merge-function ((func function-syntax-p) (smt-func func-p))
+    :returns (func func-p)
+    :short "Function for generating func-p of a single function hint."
+    :verify-guards nil
+    (b* ((func (function-syntax-fix func))
+         ((cons fun-name fun-opt-lst) func)
+         (name fun-name))
+      (make-merge-function-option-lst fun-opt-lst
+                                      (change-func smt-func :name name))))
+  (verify-guards make-merge-function
+    :hints (("Goal" :in-theory (enable function-syntax-fix function-syntax-p))))
+
+  (define merge-functions ((content function-lst-syntax-p) (hint smtlink-hint-p))
+    :returns (new-hint smtlink-hint-p)
+    :short "Merging function hints into smt-hint."
+    :measure (len content)
+    :hints (("Goal" :in-theory (enable function-lst-syntax-fix)))
+    :verify-guards nil
+    (b* ((hint (smtlink-hint-fix hint))
+         (content (function-lst-syntax-fix content))
+         ((unless (consp content)) hint)
+         ((cons first rest) content)
+         (name (car first))
+         ((smtlink-hint h) hint)
+         (exist? (hons-get name h.fast-functions))
+         (smt-func (if exist? (cdr exist?) (make-func)))
+         (new-func-lst (cons (make-merge-function first smt-func) h.functions))
+         (new-hint (change-smtlink-hint hint :functions new-func-lst)))
+      (merge-functions rest new-hint)))
+
+  (verify-guards merge-functions
+    :hints (("Goal" :in-theory (enable function-lst-syntax-fix
+                                       function-lst-syntax-p
+                                       function-syntax-p
+                                       function-syntax-fix))))
+
+
+  (define make-merge-hypothesis ((hypo hypothesis-syntax-p))
+    :returns (hp hint-pair-p)
+    :short "Generate a hint-pair for hypo"
+    :verify-guards nil
+    (b* ((hypo (hypothesis-syntax-fix hypo))
+         ((list* thm & rest) hypo))
+      (make-hint-pair :thm thm
+                      :hints (car rest))))
+
+  (verify-guards make-merge-hypothesis
+    :guard-debug t
+    :hints (("Goal" :in-theory (enable hypothesis-syntax-p hypothesis-syntax-fix hints-syntax-p))))
+
+  (define merge-hypothesis ((content hypothesis-lst-syntax-p)
+                            (hint smtlink-hint-p))
+    :returns (new-hint smtlink-hint-p)
+    :short "Merge hypothesis into hint"
+    :measure (len content)
+    :hints (("Goal" :in-theory (enable hypothesis-lst-syntax-fix)))
+    :verify-guards nil
+    (b* ((hint (smtlink-hint-fix hint))
+         (content (hypothesis-lst-syntax-fix content))
+         ((unless (consp content)) hint)
+         ((cons first rest) content)
+         ((smtlink-hint h) hint)
+         (new-hypo-lst (cons (make-merge-hypothesis first) h.hypotheses))
+         ;; It might be better to first generate the list of merging hypotheses
+         ;; and then append the old lst after them. Not sure which one takes less
+         ;; time, because I'm not sure about time complexity of
+         ;; change-smtlink-hint. Append might be expensive, too.
+         (new-hint (change-smtlink-hint hint :hypotheses new-hypo-lst)))
+      (merge-hypothesis rest new-hint)))
+  (verify-guards merge-hypothesis
+    :hints (("Goal" :in-theory (enable hypothesis-lst-syntax-p hypothesis-lst-syntax-fix))))
+
+  (define merge-main-hint ((content hints-syntax-p)
+                           (hint smtlink-hint-p))
+    :returns (new-hint smtlink-hint-p)
+    :short "Merge main-hint"
+    :verify-guards nil
+    (b* ((hint (smtlink-hint-fix hint))
+         (content (hints-syntax-fix content))
+         (new-hint (change-smtlink-hint hint :main-hint content)))
+      new-hint))
+  (verify-guards merge-main-hint
     :hints (("Goal"
-             :in-theory (enable smt-solver-cnf-p-helper smt-solver-single-cnf-p member-equal)
-             ;; :use ((:instance member-equal-preserve
-             ;;                  (x )
-             ;;                  (a )
-             ;;                  (lst )))
-             ))))
-  )
+             :in-theory (enable hints-syntax-p))))
 
-(define smt-solver-cnf-p ((term t))
-  :returns (syntax-good? booleanp)
-  :short "Recognizer for smt-solver-cnf."
-  (smt-solver-cnf-p-helper term nil))
-
-(define smt-solver-cnf-fix ((term smt-solver-cnf-p))
-  :returns (fixed-smt-cnf smt-solver-cnf-p)
-  :short "Fixing function for smt-solver-cnf."
-  (mbe :logic (if (smt-solver-cnf-p term) term nil)
-       :exec term))
-
-(defthm smt-solver-cnf-fix-idempotent-lemma
-  (equal (smt-solver-cnf-fix (smt-solver-cnf-fix x))
-         (smt-solver-cnf-fix x))
-  :hints (("Goal" :in-theory (enable smt-solver-cnf-fix))))
-
-(deffixtype smt-solver-cnf
-  :pred  smt-solver-cnf-p
-  :fix   smt-solver-cnf-fix
-  :equiv smt-solver-cnf-equiv
-  :define t
-  :forward t
-  :topic smt-solver-cnf-p)
-
-(defconst *smtlink-options*
-  '((:functions . function-lst-syntax-p)
-    (:hypothesis . hypothesis-lst-syntax-p)
-    (:main-hint . hints-syntax-p)
-    (:int-to-rat . qbooleanp)
-    (:smt-fname . qstringp)
-    (:rm-file . qbooleanp)
-    (:smt-solver-params . smt-solver-params-p)
-    (:smt-solver-cnf . smt-solver-cnf-p)))
-
-(defconst *smtlink-option-names*
-  (strip-cars *smtlink-options*))
-
-(defconst *smtlink-option-types*
-  (remove-duplicates-equal (strip-cdrs *smtlink-options*)))
-
-(define smtlink-option-type-p ((option-type t))
-  :returns (syntax-good? booleanp)
-  :short "Recoginizer for smtlink-option-type."
-  (if (member-equal option-type *smtlink-option-types*) t nil))
-
-(define smtlink-option-type-fix ((opttype smtlink-option-type-p))
-  :returns (fixed-opttype smtlink-option-type-p
-                          :hints (("Goal" :in-theory (enable
-                                                      smtlink-option-type-p))))
-  :short "Fixing function for smtlink-option-type."
-  (mbe :logic (if (smtlink-option-type-p opttype) opttype 'function-lst-syntax-p)
-       :exec opttype))
-
-(define smtlink-option-name-p ((option-name t))
-  :returns (syntax-good? booleanp)
-  :short "Recoginizer for an smtlink-option-name."
-  (if (member-equal option-name *smtlink-option-names*) t nil))
-
-(define smtlink-option-name-fix ((option smtlink-option-name-p))
-  :returns (fixed-smtlink-option-name smtlink-option-name-p)
-  :short "Fixing function for smtlink-option-name."
-  (mbe :logic (if (smtlink-option-name-p option) option ':functions)
-       :exec option))
-
-(define smtlink-option-name-lst-p ((option-lst t))
-  :returns (syntax-good? booleanp)
-  :short "Recoginizer for smtlink-option-name-lst."
-  (b* (((if (atom option-lst)) (equal option-lst nil))
-       ((cons first rest) option-lst))
-    (and (smtlink-option-name-p first)
-         (smtlink-option-name-lst-p rest))))
-
-(define smtlink-option-name-lst-fix ((option-lst smtlink-option-name-lst-p))
-  :returns (fixed-option-name-lst smtlink-option-name-lst-p
-                                  :hints (("Goal" :in-theory (enable smtlink-option-name-lst-p))))
-  :short "Fixing function for option-name-lst."
-  :verify-guards nil
-  (mbe :logic (if (atom option-lst)
-                  nil
-                (cons (smtlink-option-name-fix (car option-lst))
-                      (smtlink-option-name-lst-fix (cdr option-lst))))
-       :exec option-lst))
-(verify-guards smtlink-option-name-lst-fix
-  :hints (("Goal" :in-theory (enable smtlink-option-name-fix
-                                     smtlink-option-name-lst-fix
-                                     smtlink-option-name-p smtlink-option-name-lst-p))))
-
-(define eval-smtlink-option-type ((option-type smtlink-option-type-p) (term t))
-  :returns (type-correct? booleanp)
-  :short "Evaluating types for smtlink option body."
-  (case option-type
-    (function-lst-syntax-p (function-lst-syntax-p term))
-    (hypothesis-lst-syntax-p (hypothesis-lst-syntax-p term))
-    (hints-syntax-p (hints-syntax-p term))
-    (qbooleanp (qbooleanp term))
-    (qstringp (qstringp term))
-    (smt-solver-params-p (smt-solver-params-p term))
-    (t (smt-solver-cnf-p term))))
-
-(define smtlink-option-syntax-p ((term t) (used smtlink-option-name-lst-p))
-  :returns (mv (syntax-good? booleanp)
-               (used? smtlink-option-name-lst-p
-                      :hints (("Goal" :in-theory (enable smtlink-option-name-lst-p smtlink-option-name-p)))))
-  :short "Recoginizer for smtlink-option-syntax."
-  :verify-guards nil
-  (b* ((used (smtlink-option-name-lst-fix used))
-       ((if (equal term nil)) (mv t used))
-       ((unless (and (true-listp term) (equal (len term) 2))) (mv nil used))
-       ((cons option body-lst) term)
-       ((unless (smtlink-option-name-p option)) (mv nil used))
-       (option-type (cdr (assoc-equal option *smtlink-options*))))
-    (mv (and (not (member-equal option used))
-             (eval-smtlink-option-type option-type (car body-lst)))
-        (cons option used))))
-(verify-guards smtlink-option-syntax-p
-  :guard-debug t
-  :hints (("Goal" :in-theory (enable smtlink-option-syntax-p smtlink-option-name-p
-                                     eval-smtlink-option-type smtlink-option-name-lst-p))))
-
-(define smtlink-hint-syntax-p-helper ((term t) (used smtlink-option-name-lst-p))
-  :returns (syntax-good? booleanp)
-  :short "Helper function for smtlink-hint-syntax-p."
-  (b* (((if (atom term)) (equal term nil))
-       ((unless (and (true-listp term) (>= (len term) 2))) nil)
-       ((list* first second rest) term)
-       ((mv res new-used) (smtlink-option-syntax-p (list first second) used)))
-    (and res (smtlink-hint-syntax-p-helper rest new-used)))
-  ///
-  (defthm function-lst-syntax-p-constraint
-    (implies (and (smtlink-hint-syntax-p-helper user-hint nil)
-                  (consp user-hint)
-                  (consp (cdr user-hint)))
-             (or (equal (car user-hint) ':functions)
-                 (equal (car user-hint) ':hypothesis)
-                 (equal (car user-hint) ':main-hint)
-                 (equal (car user-hint) ':int-to-rat)
-                 (equal (car user-hint) ':smt-fname)
-                 (equal (car user-hint) ':rm-file)
-                 (equal (car user-hint) ':smt-solver-params)
-                 (equal (car user-hint) ':smt-solver-cnf)))
-    :hints (("Goal"
-             :in-theory (enable eval-smtlink-option-type
-                                smtlink-option-syntax-p
-                                smtlink-option-name-p))))
-
-  (defthm function-lst-syntax-p-of-option
-    (implies
-     (and (consp (cdr user-hint))
-          (smtlink-hint-syntax-p-helper user-hint nil)
-          (consp user-hint))
-     (and (implies (equal (car user-hint) ':functions)
-                   (function-lst-syntax-p (cadr user-hint)))
-          (implies (equal (car user-hint) ':hypothesis)
-                   (hypothesis-lst-syntax-p (cadr user-hint)))
-          (implies (equal (car user-hint) ':main-hint)
-                   (hints-syntax-p (cadr user-hint)))
-          (implies (equal (car user-hint) ':int-to-rat)
-                   (qbooleanp (cadr user-hint)))
-          (implies (equal (car user-hint) ':smt-fname)
-                   (qstringp (cadr user-hint)))
-          (implies (equal (car user-hint) ':rm-file)
-                   (qbooleanp (cadr user-hint)))
-          (implies (equal (car user-hint) ':smt-solver-params)
-                   (smt-solver-params-p (cadr user-hint)))
-          (implies (equal (car user-hint) ':smt-solver-cnf)
-                   (smt-solver-cnf-p (cadr user-hint)))))
-    :hints (("Goal"
-             :in-theory (enable smtlink-option-syntax-p
-                                eval-smtlink-option-type))))
-
-  (skip-proofs
-  (defthm smtlink-hint-syntax-preserve
-    (implies (and (smtlink-hint-syntax-p-helper term nil)
-                  (consp term))
-             (smtlink-hint-syntax-p-helper (cddr term)
-                                           nil))))
-  )
-
-(define smtlink-hint-syntax-p ((term t))
-  :returns (syntax-good? booleanp)
-  :short "Recognizer for smtlink-hint-syntax."
-  (smtlink-hint-syntax-p-helper term nil))
-
-;; Strange fixing function.
-(define smtlink-hint-syntax-fix ((term smtlink-hint-syntax-p))
-  :short "Fixing function for smtlink-hint-syntax."
-  :returns (fixed-smtlink-hint-syntax smtlink-hint-syntax-p)
-  (mbe :logic (if (smtlink-hint-syntax-p term) term nil)
-       :exec term))
-
-;; -------------------------------------------------------------------------
-
-;; (stop)
-(define make-merge-formals ((content argument-lst-syntax-p) (smt-func func-p))
-  :returns (func func-p)
-  :short "Adding user defined formals to overwrite what's already in smt-func."
-  :ignore-ok t
-  :irrelevant-formals-ok t
-  (make-func))
-
-(define make-merge-returns ((content argument-lst-syntax-p) (smf-func func-p))
-  :returns (func func-p)
-  :short "Adding user defined returns to overwrite what's already in smt-func."
-  :ignore-ok t
-  :irrelevant-formals-ok t
-  (make-func))
-
-(define make-merge-guard ((content hypothesis-lst-syntax-p) (smt-func func-p))
-  :returns (func func-p)
-  :short "Adding user defined guard to smt-func."
-  :ignore-ok t
-  :irrelevant-formals-ok t
-  (make-func))
-
-(define make-merge-more-returns ((content hypothesis-lst-syntax-p)
-                                 (smt-func func-p))
-  :returns (func func-p)
-  :short "Adding user-defined more-return theorems."
-  :ignore-ok t
-  :irrelevant-formals-ok t
-  (make-func))
-
-(define make-merge-function-option-lst ((fun-opt-lst function-option-lst-syntax-p)
-                                        (smt-fun func-p))
-  :returns (func func-p)
-  :short "Add option information into func."
-  :measure (len fun-opt-lst)
-  :hints (("Goal" :in-theory (enable function-option-lst-syntax-fix)))
-  :verify-guards nil
-  (b* ((fun-opt-lst (function-option-lst-syntax-fix fun-opt-lst))
-       (smt-fun (func-fix smt-fun))
-       ((unless (consp fun-opt-lst)) smt-fun)
-       ((cons option (cons content rest)) fun-opt-lst)
-       (new-func (case option
-                   (:formals (make-merge-formals content smt-fun))
-                   (:returns (make-merge-returns content smt-fun))
-                   (:level (change-func smt-fun :expansion-depth (cadr content)))
-                   (:guard (make-merge-guard content smt-fun))
-                   (:more-returns (make-merge-more-returns content smt-fun)))))
-    (make-merge-function-option-lst rest new-func)))
-(verify-guards make-merge-function-option-lst
-  :hints (("Goal"
-           :in-theory (enable function-option-lst-syntax-fix
-                              function-option-lst-syntax-p
-                              function-option-lst-syntax-p-helper
-                              qnatp)
-           :use ((:instance function-option-lst-syntax-p-of-option)
-                 (:instance function-option-lst-syntax-p-constraint))))) 
-
-(define make-merge-function ((func function-syntax-p) (smt-fun func-p))
-  :returns (func func-p)
-  :short "Function for generating func-p of a single function hint."
-  :verify-guards nil
-  (b* ((func (function-syntax-fix func))
-       ((cons fun-name fun-opt-lst) func)
-       (name fun-name))
-    (make-merge-function-option-lst fun-opt-lst
-                                    (change-func smt-fun :name name))))
-(verify-guards make-merge-function
-  :hints (("Goal" :in-theory (enable function-syntax-fix function-syntax-p))))
-
-(define merge-functions ((content function-lst-syntax-p) (hint smtlink-hint-p))
-  :returns (new-hint smtlink-hint-p)
-  :short "Merging function hints into smt-hint."
-  :measure (len content)
-  :hints (("Goal" :in-theory (enable function-lst-syntax-fix)))
-  :verify-guards nil
-  (b* ((hint (smtlink-hint-fix hint))
-       (content (function-lst-syntax-fix content))
-       ((unless (consp content)) hint)
-       ((cons first rest) content)
-       (name (car first))
-       ((smtlink-hint h) hint)
-       (exist? (hons-get name h.fast-functions))
-       (smt-fun (if exist? (cdr exist?) (make-func)))
-       (new-func-lst (cons (make-merge-function first smt-fun) h.functions))
-       (new-hint (change-smtlink-hint hint :functions new-func-lst)))
-    (merge-functions rest new-hint)))
-
-(verify-guards merge-functions
-  :hints (("Goal" :in-theory (enable function-lst-syntax-fix
-                                     function-lst-syntax-p
-                                     function-syntax-p
-                                     function-syntax-fix))))
-
-
-(define make-merge-hypothesis ((hypo hypothesis-syntax-p))
-  :returns (hp hint-pair-p)
-  :short "Generate a hint-pair for hypo"
-  :verify-guards nil
-  (b* ((hypo (hypothesis-syntax-fix hypo))
-       ((cons thm (cons & rest)) hypo))
-    (make-hint-pair :thm thm
-                    :hints (car rest))))
-(verify-guards make-merge-hypothesis
-  :guard-debug t
-  :hints (("Goal" :in-theory (enable hypothesis-syntax-p hypothesis-syntax-fix))))
-
-(define merge-hypothesis ((content hypothesis-lst-syntax-p)
+  (define set-int-to-rat ((content qbooleanp)
                           (hint smtlink-hint-p))
-  :returns (new-hint smtlink-hint-p)
-  :short "Merge hypothesis into hint"
-  :measure (len content)
-  :hints (("Goal" :in-theory (enable hypothesis-lst-syntax-fix)))
-  :verify-guards nil
-  (b* ((hint (smtlink-hint-fix hint))
-       (content (hypothesis-lst-syntax-fix content))
-       ((unless (consp content)) hint)
-       ((cons first rest) content)
-       ((smtlink-hint h) hint)
-       (new-hypo-lst (cons (make-merge-hypothesis first) h.hypotheses))
-       ;; It might be better to first generate the list of merging hypotheses
-       ;; and then append the old lst after them. Not sure which one takes less
-       ;; time, because I'm not sure about time complexity of
-       ;; change-smtlink-hint. Append might be expensive, too.
-       (new-hint (change-smtlink-hint hint :hypotheses new-hypo-lst)))
-    (merge-hypothesis rest new-hint)))
-(verify-guards merge-hypothesis
-  :hints (("Goal" :in-theory (enable hypothesis-lst-syntax-p hypothesis-lst-syntax-fix))))
+    :returns (new-hint smtlink-hint-p)
+    :short "Set :int-to-rat based on user hint."
+    :verify-guards nil
+    (b* ((hint (smtlink-hint-fix hint))
+         (content (qboolean-fix content))
+         (new-hint (change-smtlink-hint hint :int-to-rat (cadr content))))
+      new-hint))
 
-(define merge-main-hint ((content hints-syntax-p)
-                         (hint smtlink-hint-p))
-  :returns (new-hint smtlink-hint-p)
-  :short "Merge main-hint"
-  :verify-guards nil
-  (b* ((hint (smtlink-hint-fix hint))
-       (content (hints-syntax-fix content))
-       (new-hint (change-smtlink-hint hint :main-hint content)))
-    new-hint))
-(verify-guards merge-main-hint
-  :hints (("Goal"
-           :in-theory (enable hints-syntax-p))))
+  (verify-guards set-int-to-rat
+    :hints (("Goal"
+             :in-theory (enable qbooleanp qboolean-fix))))
 
-(define set-int-to-rat ((content qbooleanp)
-                        (hint smtlink-hint-p))
-  :returns (new-hint smtlink-hint-p)
-  :short "Set :int-to-rat based on user hint."
-  :verify-guards nil
-  (b* ((hint (smtlink-hint-fix hint))
-       (content (qboolean-fix content))
-       (new-hint (change-smtlink-hint hint :int-to-rat (cadr content))))
-    new-hint))
+  (define set-fname ((content qstringp) (hint smtlink-hint-p))
+    :returns (new-hint smtlink-hint-p)
+    :short "Set :smt-fname."
+    :verify-guards nil
+    (b* ((hint (smtlink-hint-fix hint))
+         (content (qstring-fix content))
+         (new-hint (change-smtlink-hint hint :smt-fname (cadr content))))
+      new-hint))
+  (verify-guards set-fname
+    :hints (("Goal"
+             :in-theory (enable qstringp qstring-fix))))
 
-(verify-guards set-int-to-rat
-  :hints (("Goal"
-           :in-theory (enable qbooleanp qboolean-fix))))
+  (define set-rm-file ((content qbooleanp)
+                       (hint smtlink-hint-p))
+    :returns (new-hint smtlink-hint-p)
+    :short "Set :rm-file"
+    :verify-guards nil
+    (b* ((hint (smtlink-hint-fix hint))
+         (content (qboolean-fix content))
+         (new-hint (change-smtlink-hint hint :rm-file (cadr content))))
+      new-hint))
+  (verify-guards set-rm-file
+    :hints (("Goal"
+             :in-theory (enable qbooleanp qboolean-fix))))
 
-(define set-fname ((content qstringp) (hint smtlink-hint-p))
-  :returns (new-hint smtlink-hint-p)
-  :short "Set :smt-fname."
-  :verify-guards nil
-  (b* ((hint (smtlink-hint-fix hint))
-       (content (qstring-fix content))
-       (new-hint (change-smtlink-hint hint :smt-fname (cadr content))))
-    new-hint))
-(verify-guards set-fname
-  :hints (("Goal"
-           :in-theory (enable qstringp qstring-fix))))
+  (define set-smt-solver-params ((content smt-solver-params-p)
+                                 (hint smtlink-hint-p))
+    :returns (new-hint smtlink-hint-p)
+    :short "Set :smt-params"
+    :verify-guards nil
+    (b* ((hint (smtlink-hint-fix hint))
+         (content (smt-solver-params-fix content))
+         (new-hint (change-smtlink-hint hint :smt-params content)))
+      new-hint))
+  (verify-guards set-smt-solver-params
+    :hints (("Goal"
+             :in-theory (enable smt-solver-params-p smt-solver-params-fix))))
 
-(define set-rm-file ((content qbooleanp)
-                     (hint smtlink-hint-p))
-  :returns (new-hint smtlink-hint-p)
-  :short "Set :rm-file"
-  :verify-guards nil
-  (b* ((hint (smtlink-hint-fix hint))
-       (content (qboolean-fix content))
-       (new-hint (change-smtlink-hint hint :rm-file (cadr content))))
-    new-hint))
-(verify-guards set-rm-file
-  :hints (("Goal"
-           :in-theory (enable qbooleanp qboolean-fix))))
+  (define merge-smt-solver-cnf ((content smt-solver-cnf-p)
+                                (hint smtlink-hint-p))
+    :returns (new-hint smtlink-hint-p)
+    :short "Set :smt-cnf"
+    :measure (len content)
+    :hints (("Goal" :in-theory (enable smt-solver-cnf-fix)))
+    :verify-guards nil
+    (b* ((hint (smtlink-hint-fix hint))
+         (content (smt-solver-cnf-fix content))
+         ((unless (consp content)) hint)
+         ((cons option (cons str rest)) content)
+         ((smtlink-hint h) hint)
+         (new-cnf (case option
+                    (:interface-dir
+                     (change-smtlink-config h.smt-cnf
+                                            :interface-dir (cadr str)))
+                    (:SMT-files-dir
+                     (change-smtlink-config h.smt-cnf
+                                            :SMT-files-dir (cadr str)))
+                    (:SMT-module
+                     (change-smtlink-config h.smt-cnf
+                                            :SMT-module (cadr str)))
+                    (:SMT-class
+                     (change-smtlink-config h.smt-cnf
+                                            :SMT-class (cadr str)))
+                    (:SMT-cmd
+                     (change-smtlink-config h.smt-cnf
+                                            :SMT-cmd (cadr str)))
+                    (t
+                     (change-smtlink-config h.smt-cnf
+                                            :file-format (cadr str)))))
+         (new-hint (change-smtlink-hint hint :smt-cnf new-cnf)))
+      (merge-smt-solver-cnf rest new-hint)))
 
-(define set-smt-solver-params ((content smt-solver-params-p)
-                               (hint smtlink-hint-p))
-  :returns (new-hint smtlink-hint-p)
-  :short "Set :smt-params"
-  :verify-guards nil
-  (b* ((hint (smtlink-hint-fix hint))
-       (content (smt-solver-params-fix content))
-       (new-hint (change-smtlink-hint hint :smt-params content)))
-    new-hint))
-(verify-guards set-smt-solver-params
-  :hints (("Goal"
-           :in-theory (enable smt-solver-params-p smt-solver-params-fix))))
+  (verify-guards merge-smt-solver-cnf
+    :guard-debug t
+    :hints (("Goal" :in-theory (enable smt-solver-cnf-fix smt-solver-cnf-p
+                                       smt-solver-cnf-p-helper)
+             :use ((:instance stringp-of-cadr)))))
 
-(define merge-smt-solver-cnf ((content smt-solver-cnf-p)
-                              (hint smtlink-hint-p))
-  :returns (new-hint smtlink-hint-p)
-  :short "Set :smt-cnf"
-  :measure (len content)
-  :hints (("Goal" :in-theory (enable smt-solver-cnf-fix)))
-  :verify-guards nil
-  (b* ((hint (smtlink-hint-fix hint))
-       (content (smt-solver-cnf-fix content))
-       ((unless (consp content)) hint)
-       ((cons option (cons str rest)) content)
-       ((smtlink-hint h) hint)
-       (new-cnf (case option
-                  (:interface-dir
-                   (change-smtlink-config h.smt-cnf
-                                          :interface-dir (cadr str)))
-                  (:SMT-files-dir
-                   (change-smtlink-config h.smt-cnf
-                                          :SMT-files-dir (cadr str)))
-                  (:SMT-module
-                   (change-smtlink-config h.smt-cnf
-                                          :SMT-module (cadr str)))
-                  (:SMT-class
-                   (change-smtlink-config h.smt-cnf
-                                          :SMT-class (cadr str)))
-                  (:SMT-cmd
-                   (change-smtlink-config h.smt-cnf
-                                          :SMT-cmd (cadr str)))
-                  (t
-                   (change-smtlink-config h.smt-cnf
-                                          :file-format (cadr str)))))
-       (new-hint (change-smtlink-hint hint :smt-cnf new-cnf)))
-    (merge-smt-solver-cnf rest new-hint)))
+  (define combine-hints ((user-hint smtlink-hint-syntax-p) (hint smtlink-hint-p))
+    :returns (combined-hint smtlink-hint-p)
+    :hints (("Goal" :in-theory (enable smtlink-hint-syntax-fix)))
+    :measure (len user-hint)
+    :short "Combining user-hints into smt-hint."
+    :verify-guards nil
+    (b* ((hint (smtlink-hint-fix hint))
+         (user-hint (smtlink-hint-syntax-fix user-hint))
+         ((unless (consp user-hint)) hint)
+         ((cons option (cons second rest)) user-hint)
+         ((smtlink-hint h) hint)
+         (fast-funcs (make-alist-fn-lst h.functions))
+         (new-hint (case option
+                     (:functions (with-fast-alist fast-funcs
+                                   (merge-functions second
+                                                    (change-smtlink-hint
+                                                     hint
+                                                     :fast-functions fast-funcs))))
+                     (:hypothesis (merge-hypothesis second hint))
+                     (:main-hint (merge-main-hint second hint))
+                     (:int-to-rat (set-int-to-rat second hint))
+                     (:smt-fname (set-fname second hint))
+                     (:rm-file (set-rm-file second hint))
+                     (:smt-solver-params (set-smt-solver-params second hint))
+                     (t (merge-smt-solver-cnf second hint)))))
+      (combine-hints rest new-hint)))
 
-(verify-guards merge-smt-solver-cnf
-  :guard-debug t
-  :hints (("Goal" :in-theory (enable smt-solver-cnf-fix smt-solver-cnf-p
-                                     smt-solver-cnf-p-helper)
-           :use ((:instance stringp-of-cadr)))))
+  (defthm true-listp-of-smtlink-hint-syntax-p
+    (implies (smtlink-hint-syntax-p x)
+             (true-listp x))
+    :hints (("Goal" :in-theory (enable smtlink-hint-syntax-p
+                                       smtlink-hint-syntax-p-helper))))
+  (defthm crock
+    (implies (and (true-listp x) (not (consp (cdr x)))) (not (cdr x))))
 
-(define combine-hints ((user-hint smtlink-hint-syntax-p) (hint smtlink-hint-p))
-  :returns (combined-hint smtlink-hint-p)
-  :hints (("Goal" :in-theory (enable smtlink-hint-syntax-fix)))
-  :measure (len user-hint)
-  :short "Combining user-hints into smt-hint."
-  :verify-guards nil
-  (b* ((hint (smtlink-hint-fix hint))
-       (user-hint (smtlink-hint-syntax-fix user-hint))
-       ((unless (consp user-hint)) hint)
-       ((cons option (cons second rest)) user-hint)
-       ((smtlink-hint h) hint)
-       (fast-funcs (make-alist-fn-lst h.functions))
-       (new-hint (case option
-                   (:functions (with-fast-alist fast-funcs
-                                 (merge-functions second
-                                                  (change-smtlink-hint
-                                                   hint
-                                                   :fast-functions fast-funcs))))
-                   (:hypothesis (merge-hypothesis second hint))
-                   (:main-hint (merge-main-hint second hint))
-                   (:int-to-rat (set-int-to-rat second hint))
-                   (:smt-fname (set-fname second hint))
-                   (:rm-file (set-rm-file second hint))
-                   (:smt-solver-params (set-smt-solver-params second hint))
-                   (t (merge-smt-solver-cnf second hint)))))
-    (combine-hints rest new-hint)))
-
-(defthm true-listp-of-smtlink-hint-syntax-p
-  (implies (smtlink-hint-syntax-p x)
-           (true-listp x))
-  :hints (("Goal" :in-theory (enable smtlink-hint-syntax-p
-                                     smtlink-hint-syntax-p-helper))))
-(defthm crock
-  (implies (and (true-listp x) (not (consp (cdr x)))) (not (cdr x))))
-
-(verify-guards combine-hints
-  :guard-debug t
-  :hints (("Goal"
-           :in-theory (enable smtlink-hint-syntax-fix smtlink-hint-syntax-p smtlink-hint-syntax-p-helper)
-           :use ((:instance true-listp-of-smtlink-hint-syntax-p (x user-hint))
-                 (:instance crock (x user-hint))
-                 (:instance function-lst-syntax-p-of-option)
-                 (:instance function-lst-syntax-p-constraint)
-                 (:instance smtlink-hint-syntax-preserve)))))
+  (verify-guards combine-hints
+    :guard-debug t
+    :hints (("Goal"
+             :in-theory (enable smtlink-hint-syntax-fix smtlink-hint-syntax-p smtlink-hint-syntax-p-helper)
+             :use ((:instance true-listp-of-smtlink-hint-syntax-p (x user-hint))
+                   (:instance crock (x user-hint))
+                   (:instance function-lst-syntax-p-of-option)
+                   (:instance function-lst-syntax-p-constraint)
+                   (:instance smtlink-hint-syntax-preserve)))))
 
   (define process-hint ((cl pseudo-term-listp) (user-hint t))
     :returns (subgoal-lst pseudo-term-list-listp)
-    :enabled t
     (b* ((cl (pseudo-term-list-fix cl))
          (- (cw "user-hint: ~q0" user-hint))
          ((unless (smtlink-hint-syntax-p user-hint))
@@ -1088,6 +1283,7 @@
 
   (def-join-thms ev-process-hint)
 
+  (local (in-theory (enable process-hint)))
   (defthm correctness-of-process-hint
     (implies (and (pseudo-term-listp cl)
                   (alistp b)
@@ -1104,4 +1300,4 @@
   ;;   expansion and transformation.
   (defmacro Smtlink (clause hint)
     `(process-hint ,clause ,hint))
-;;  )
+  )
